coq/Monad.v
@@ -1,0 +1,182 @@
+(* From coq-ext-lib/theories/structures/Functor / Applicative / Monad *)
+
+Set Implicit Arguments.
+Set Strict Implicit.
+Set Universe Polymorphism.
+
+Declare Scope monad_scope.
+
+Polymorphic Class Functor@{d c} (F : Type@{d} -> Type@{c}) : Type :=
+{ fmap : forall {A B : Type@{d}}, (A -> B) -> F A -> F B }.
+
+Polymorphic Definition ID@{d} {T : Type@{d}} (f : T -> T) : Prop :=
+  forall x : T, f x = x.
+
+Module FunctorNotation.
+  Notation "f <$> x" := (@fmap _ _ _ _ f x) (at level 52, left associativity).
+End FunctorNotation.
+
+
+Class Applicative@{d c} (T : Type@{d} -> Type@{c}) :=
+{ pure : forall {A : Type@{d}}, A -> T A
+; ap : forall {A B : Type@{d}}, T (A -> B) -> T A -> T B
+}.
+
+Module ApplicativeNotation.
+  Notation "f <*> x" := (ap f x) (at level 52, left associativity).
+End ApplicativeNotation.
+Import ApplicativeNotation.
+
+Section applicative.
+  Definition liftA@{d c} {T : Type@{d} -> Type@{c}} {AT:Applicative@{d c} T} {A B : Type@{d}} (f:A -> B) (aT:T A) : T B := pure f <*> aT.
+  Definition liftA2@{d c} {T : Type@{d} -> Type@{c}} {AT:Applicative@{d c} T} {A B C : Type@{d}} (f:A -> B -> C) (aT:T A) (bT:T B) : T C := liftA f aT <*> bT.
+End applicative.
+
+Section Instances.
+
+Universe d c.
+Context (T : Type@{d} -> Type@{c}) {AT : Applicative T}.
+
+Global Instance Functor_Applicative@{} : Functor T :=
+{ fmap := @liftA _ _ }.
+
+End Instances.
+
+
+Class Monad@{d c} (m : Type@{d} -> Type@{c}) : Type :=
+{ ret : forall {t : Type@{d}}, t -> m t
+; bind : forall {t u : Type@{d}}, m t -> (t -> m u) -> m u
+}.
+
+Section monadic.
+
+  Definition liftM@{d c}
+              {m : Type@{d} -> Type@{c}}
+              {M : Monad m}
+              {T U : Type@{d}} (f : T -> U) : m T -> m U :=
+    fun x => bind x (fun x => ret (f x)).
+
+  Definition liftM2@{d c}
+              {m : Type@{d} -> Type@{c}}
+              {M : Monad m}
+              {T U V : Type@{d}} (f : T -> U -> V) : m T -> m U -> m V :=
+    Eval cbv beta iota zeta delta [ liftM ] in
+      fun x y => bind x (fun x => liftM (f x) y).
+
+  Definition liftM3@{d c}
+              {m : Type@{d} -> Type@{c}}
+              {M : Monad m}
+              {T U V W : Type@{d}} (f : T -> U -> V -> W) : m T -> m U -> m V -> m W :=
+    Eval cbv beta iota zeta delta [ liftM2 ] in
+      fun x y z => bind x (fun x => liftM2 (f x) y z).
+
+  Definition apM@{d c}
+              {m : Type@{d} -> Type@{c}}
+              {M : Monad m}
+              {A B : Type@{d}} (fM:m (A -> B)) (aM:m A) : m B :=
+    bind fM (fun f => liftM f aM).
+
+  (* Left-to-right composition of Kleisli arrows. *)
+  Definition mcompose@{c d}
+             {m:Type@{d}->Type@{c}}
+             {M: Monad m}
+             {T U V:Type@{d}}
+             (f: T -> m U) (g: U -> m V): (T -> m V) :=
+    fun x => bind (f x) g.
+
+  Definition join@{d c} {m : Type@{d} -> Type@{c}} {a} `{Monad m} : m (m a) -> m a :=
+    fun x => bind x (fun y => y).
+
+End monadic.
+
+Module MonadBaseNotation.
+
+  Delimit Scope monad_scope with monad.
+
+  Notation "c >>= f" := (@bind _ _ _ _ c f) (at level 58, left associativity) : monad_scope.
+  Notation "f =<< c" := (@bind _ _ _ _ c f) (at level 61, right associativity) : monad_scope.
+  Notation "f >=> g" := (@mcompose _ _ _ _ _ f g) (at level 61, right associativity) : monad_scope.
+
+  Notation "e1 ;; e2" := (@bind _ _ _ _ e1%monad (fun _ => e2%monad))%monad
+    (at level 61, right associativity) : monad_scope.
+
+End MonadBaseNotation.
+
+Module MonadNotation.
+
+  Export MonadBaseNotation.
+
+  Notation "x <- c1 ;; c2" := (@bind _ _ _ _ c1 (fun x => c2))
+    (at level 61, c1 at next level, right associativity) : monad_scope.
+
+  Notation "' pat <- c1 ;; c2" :=
+    (@bind _ _ _ _ c1 (fun x => match x with pat => c2 end))
+    (at level 61, pat pattern, c1 at next level, right associativity) : monad_scope.
+
+End MonadNotation.
+
+Module MonadLetNotation.
+
+  Export MonadBaseNotation.
+
+  Notation "'let*' p ':=' c1 'in' c2" := (@bind _ _ _ _ c1 (fun p => c2))
+    (at level 61, p as pattern, c1 at next level, right associativity) : monad_scope.
+
+End MonadLetNotation.
+
+Section Instances.
+
+Universe d c.
+Context (m : Type@{d} -> Type@{c}) {M : Monad m}.
+
+Global Instance Functor_Monad@{} : Functor m :=
+{ fmap := @liftM _ _ }.
+
+Global Instance Applicative_Monad@{} : Applicative m :=
+{ pure := @ret _ _
+; ap := @apM _ _
+}.
+
+End Instances.
+
+(* ---------------- Alternative ---------------- *)
+
+Class Alternative@{d c} (m : Type@{d} -> Type@{c}) : Type :=
+  { empty  : forall {t : Type@{d}}, m t 
+  ; choose : forall {t : Type@{d}}, m t -> m t -> m t
+  }.
+
+Module AlternativeNotation.
+  Notation "f1 <|> f2" := (@choose _ _ _ f1 f2) (at level 52, left associativity).
+End AlternativeNotation.
+
+
+(* ---------------- Instances ---------------- *)
+
+(* list monad *)
+
+Require Import Coq.Lists.List.
+
+Global Instance Functor_list : Functor list :=
+{ fmap := map }.
+
+Global Instance Monad_list : Monad list :=
+{ ret  := fun _ x => x :: nil; 
+  bind := fun _ _ x f =>  flat_map f x
+}.
+
+Global Instance Alternative_list : Alternative list :=
+  { empty := @nil ;
+    choose := @app
+  }.
+
+(* Error monad *)
+
+Global Instance Monad_error {E} : Monad (sum E) :=
+  { ret := fun _ x => inr x ;
+    bind := fun _ _ x k => match x with 
+                        | inl y => inl y
+                        | inr v => k v
+                        end }. 
+
+                                       
